feat: add support for Diffie-Hellman

src/DY.Core.Bytes.Type.fst
@@ -25,13 +25,14 @@ open DY.Core.Label.Type
 /// At the end, this usage string may play a role in the security proof
 /// via the protocol invariants.
 
-type usage_ (bytes:Type0) =
-  | SigKey: tag:string -> usage_ bytes
-  | SigNonce: usage_ bytes
-  | PkdecKey: tag:string -> usage_ bytes
-  | PkNonce: usage_ bytes
-  | AeadKey: tag:string -> usage_ bytes
-  | NoUsage: usage_ bytes // baked-in None
+type usage =
+  | SigKey: tag:string -> usage
+  | SigNonce: usage
+  | PkdecKey: tag:string -> usage
+  | PkNonce: usage
+  | AeadKey: tag:string -> usage
+  | DhKey: tag:string -> usage
+  | NoUsage: usage // baked-in None
 
 /// The bytes term.
 /// It is similar to the one you would find in other symbolic analysis tools.
@@ -46,11 +47,11 @@ type usage_ (bytes:Type0) =
 /// (e.g. the plaintext if the bytes is an encryption with the correct key).
 /// This allows us to reason with F*'s logical equality (`==`).
 
-type bytes =
+and bytes =
   // Public values (strings, numbers, ...)
   | Literal: FStar.Seq.seq FStar.UInt8.t -> bytes
   // Randomly generated numbers. `time` is used to ensure two random numbers are distinct.
-  | Rand: usage:usage_ bytes -> label:label -> len:nat{len <> 0} -> time:nat -> bytes
+  | Rand: usage:usage -> label:label -> len:nat{len <> 0} -> time:nat -> bytes
 
   // Concatenation
   | Concat: left:bytes -> right:bytes -> bytes
@@ -69,6 +70,98 @@ type bytes =
   // Hash
   | Hash: msg:bytes -> bytes
 
+  // Diffie-Hellman
+  | DhPub: sk:bytes -> bytes
+  | Dh: sk:bytes -> pk:bytes -> bytes
   // ...
 
-type usage = usage_ bytes
+open DY.Core.Internal.Ord
+
+val encode_usage: usage -> list int
+val encode_bytes: bytes -> list int
+let rec encode_usage usg =
+  match usg with
+  | SigKey tag -> 0::(encode_list [encode tag])
+  | SigNonce -> 1::[]
+  | PkdecKey tag -> 2::(encode_list [encode tag])
+  | PkNonce -> 3::[]
+  | AeadKey tag -> 4::(encode_list [encode tag])
+  | DhKey tag -> 5::(encode_list [encode tag])
+  | NoUsage -> 6::[]
+and encode_bytes b =
+  match b with
+  | Literal l -> 0::(encode_list [encode l])
+  | Rand usg lab len time -> 1::(encode_list [encode_usage usg; encode lab; encode (len <: nat); encode time])
+  | Concat left right -> 2::(encode_list [encode_bytes left; encode_bytes right])
+  | AeadEnc key nonce msg ad -> 3::(encode_list [encode_bytes key; encode_bytes nonce; encode_bytes msg; encode_bytes ad])
+  | Pk sk -> 4::(encode_list [encode_bytes sk])
+  | PkEnc pk nonce msg -> 5::(encode_list [encode_bytes pk; encode_bytes nonce; encode_bytes msg])
+  | Vk sk -> 6::(encode_list [encode_bytes sk])
+  | Sign sk nonce msg -> 7::(encode_list [encode_bytes sk; encode_bytes nonce; encode_bytes msg])
+  | Hash msg -> 8::(encode_list [encode_bytes msg])
+  | DhPub sk -> 9::(encode_list [encode_bytes sk])
+  | Dh sk pk -> 10::(encode_list [encode_bytes sk; encode_bytes pk])
+
+#push-options "--z3rlimit 50"
+val encode_usage_inj: usg1:usage -> usg2:usage -> Lemma (requires encode_usage usg1 == encode_usage usg2) (ensures usg1 == usg2)
+val encode_bytes_inj: b1:bytes -> b2:bytes -> Lemma (requires encode_bytes b1 == encode_bytes b2) (ensures b1 == b2)
+let rec encode_usage_inj usg1 usg2 =
+  introduce forall b1 b2. b1 << usg1 /\ b2 << usg2 /\ encode_bytes b1 == encode_bytes b2 ==> b1 == b2 with (
+    introduce _ ==> _ with _. (
+      encode_bytes_inj b1 b2
+    )
+  );
+  encode_inj_forall (list (list int)) ();
+  encode_inj_forall string ()
+and encode_bytes_inj b1 b2 =
+  introduce forall usg1 usg2. usg1 << b1 /\ usg2 << b2 /\ encode_usage usg1 == encode_usage usg2 ==> usg1 == usg2 with (
+    introduce _ ==> _ with _. (
+      encode_usage_inj usg1 usg2
+    )
+  );
+  // Do not introduce injectivity on bytes,
+  // this makes the SMT go crazy.
+  // Instead do the manual (but factorized) match below
+  //introduce forall b1' b2'. b1' << b1 /\ b2' << b2 /\ encode_bytes b1' == encode_bytes b2' ==> b1' == b2' with (
+  //  introduce _ ==> _ with _. (
+  //    encode_bytes_inj b1' b2'
+  //  )
+  //);
+  encode_inj_forall (list (list int)) ();
+  encode_inj_forall (FStar.Seq.seq FStar.UInt8.t) ();
+  encode_inj_forall label ();
+  encode_inj_forall nat ();
+  match b1, b2 with
+  | Literal _, Literal _ -> ()
+  | Rand _ _ _ _, Rand _ _ _ _ -> ()
+  | Pk x1, Pk y1
+  | Vk x1, Vk y1
+  | Hash x1, Hash y1
+  | DhPub x1, DhPub y1 ->
+    encode_bytes_inj x1 y1
+  | Concat x1 x2, Concat y1 y2
+  | Dh x1 x2, Dh y1 y2 ->
+    encode_bytes_inj x1 y1;
+    encode_bytes_inj x2 y2
+  | PkEnc x1 x2 x3, PkEnc y1 y2 y3
+  | Sign x1 x2 x3, Sign y1 y2 y3 ->
+    encode_bytes_inj x1 y1;
+    encode_bytes_inj x2 y2;
+    encode_bytes_inj x3 y3
+  | AeadEnc x1 x2 x3 x4, AeadEnc y1 y2 y3 y4 ->
+    encode_bytes_inj x1 y1;
+    encode_bytes_inj x2 y2;
+    encode_bytes_inj x3 y3;
+    encode_bytes_inj x4 y4
+  | _, _ -> assert(False)
+#pop-options
+
+instance integer_encodable_usage: integer_encodable usage = {
+  encode = encode_usage;
+  encode_inj = encode_usage_inj;
+}
+
+instance integer_encodable_bytes: integer_encodable bytes = {
+  encode = encode_bytes;
+  encode_inj = encode_bytes_inj;
+}
