src/DY.Core.Internal.Ord.fst
@@ -1,0 +1,225 @@
+module DY.Core.Internal.Ord
+
+open FStar.List.Tot
+
+/// This module defines a typeclass `integer_encodable`,
+/// for types that can be (injectively) encoded as a list of integers,
+/// and defines a total order `is_less_than` for instances of this typeclass.
+///
+/// This will be useful to define an order on `bytes` terms,
+/// to normalize cryptographic functions that feature commutativity properties
+/// (such as Diffie-Hellman or XOR).
+
+class integer_encodable (t:Type) = {
+  encode: t -> list int;
+  encode_inj: x:t -> y:t -> Lemma
+    (requires encode x == encode y)
+    (ensures x == y)
+  ;
+}
+
+val encode_inj_forall:
+  t:Type -> {|integer_encodable t|} ->
+  unit ->
+  Lemma
+  (forall (x:t) (y:t). encode x == encode y ==> x == y)
+let encode_inj_forall t #ie () =
+  FStar.Classical.forall_intro_2 (FStar.Classical.move_requires_2 (encode_inj #t))
+
+val is_less_than_aux:
+  list int -> list int ->
+  bool
+let rec is_less_than_aux x y =
+  match x, y with
+  | [], [] -> true
+  | [], hy::ty -> true
+  | hx::tx, [] -> false
+  | hx::tx, hy::ty ->
+    hx < hy || (hx = hy && is_less_than_aux tx ty)
+
+val is_less_than:
+  #t:Type -> {|integer_encodable t|} ->
+  t -> t ->
+  bool
+let is_less_than #t #ie x y =
+  is_less_than_aux (encode x) (encode y)
+
+val is_less_than_aux_total:
+  x:list int -> y:list int ->
+  Lemma (x `is_less_than_aux` y \/ y `is_less_than_aux` x)
+let rec is_less_than_aux_total x y =
+  match x, y with
+  | [], [] -> ()
+  | hx::tx, [] -> ()
+  | [], hy::ty -> ()
+  | hx::tx, hy::ty -> is_less_than_aux_total tx ty
+
+val is_less_than_aux_refl:
+  x:list int ->
+  Lemma (x `is_less_than_aux` x)
+let rec is_less_than_aux_refl x =
+  match x with
+  | [] -> ()
+  | hx::tx -> is_less_than_aux_refl tx
+
+val is_less_than_aux_trans:
+  x:list int -> y:list int -> z:list int ->
+  Lemma
+  (requires x `is_less_than_aux` y /\ y `is_less_than_aux` z)
+  (ensures x `is_less_than_aux` z)
+let rec is_less_than_aux_trans x y z =
+  match x, y, z with
+  | [], _ , _ -> ()
+  | hx::tx, [], _ -> ()
+  | hx::tx, hy::ty, [] -> ()
+  | hx::tx, hy::ty, hz::tz ->
+    if hx = hy && hy = hz then
+      is_less_than_aux_trans tx ty tz
+    else ()
+
+val is_less_than_aux_antisym:
+  x:list int -> y:list int ->
+  Lemma
+  (requires x `is_less_than_aux` y /\ y `is_less_than_aux` x)
+  (ensures x == y)
+let rec is_less_than_aux_antisym x y =
+  match x, y with
+  | [], [] -> ()
+  | hx::tx, [] -> assert(False)
+  | [], hy::ty -> assert(False)
+  | hx::tx, hy::ty ->
+    is_less_than_aux_antisym tx ty
+
+val is_less_than_total:
+  #t:Type -> {|integer_encodable t|} ->
+  x:t -> y:t ->
+  Lemma (x `is_less_than` y \/ y `is_less_than` x)
+let is_less_than_total x y =
+  is_less_than_aux_total (encode x) (encode y)
+
+val is_less_than_refl:
+  #t:Type -> {|integer_encodable t|} ->
+  x:t ->
+  Lemma (x `is_less_than` x)
+let is_less_than_refl x =
+  is_less_than_aux_refl (encode x)
+
+val is_less_than_trans:
+  #t:Type -> {|integer_encodable t|} ->
+  x:t -> y:t -> z:t ->
+  Lemma
+  (requires x `is_less_than` y /\ y `is_less_than` z)
+  (ensures x `is_less_than` z)
+let is_less_than_trans x y z =
+  is_less_than_aux_trans (encode x) (encode y) (encode z)
+
+val is_less_than_antisym:
+  #t:Type -> {|integer_encodable t|} ->
+  x:t -> y:t ->
+  Lemma
+  (requires x `is_less_than` y /\ y `is_less_than` x)
+  (ensures x == y)
+let is_less_than_antisym x y =
+  is_less_than_aux_antisym (encode x) (encode y);
+  encode_inj x y
+
+instance integer_encodable_list_int: integer_encodable (list int) = {
+  encode = (fun x -> x);
+  encode_inj = (fun x y -> ());
+}
+
+val encode_pair:
+  #t1:Type -> #t2:Type ->
+  {|integer_encodable t1|} -> {|integer_encodable t2|} ->
+  t1 -> t2 ->
+  list int
+let encode_pair x1 x2 =
+  let l1 = encode x1 in
+  let l2 = encode x2 in
+  (List.Tot.length l1)::l1@l2
+
+val encode_pair_inj:
+  #t1:Type -> #t2:Type ->
+  {|integer_encodable t1|} -> {|integer_encodable t2|} ->
+  x1:t1 -> x2:t2 ->
+  y1:t1 -> y2:t2 ->
+  Lemma
+  (requires encode_pair x1 x2 == encode_pair y1 y2)
+  (ensures x1 == y1 /\ x2 == y2)
+let encode_pair_inj x1 x2 y1 y2 =
+  List.Tot.Properties.append_length_inv_head (encode x1) (encode x2) (encode y1) (encode y2);
+  encode_inj x1 y1;
+  encode_inj x2 y2
+
+val encode_list:
+  #t:Type ->
+  {|integer_encodable t|} ->
+  list t ->
+  list int
+let encode_list l =
+  List.Tot.fold_right encode_pair (List.Tot.map encode l) []
+
+val encode_list_inj:
+  #t:Type ->
+  {|integer_encodable t|} ->
+  x:list t -> y:list t ->
+  Lemma
+  (requires encode_list x == encode_list y)
+  (ensures x == y)
+let rec encode_list_inj x y =
+  match x, y with
+  | [], [] -> ()
+  | hx::tx, [] -> assert(False)
+  | [], hy::ty -> assert(False)
+  | hx::tx, hy::ty ->
+    encode_pair_inj hx (encode_list tx) hy (encode_list ty);
+    encode_list_inj tx ty
+
+instance integer_encodable_list (t:Type) {|integer_encodable t|}: integer_encodable (list t) = {
+  encode = encode_list;
+  encode_inj = encode_list_inj;
+}
+
+instance integer_encodable_nat: integer_encodable nat = {
+  encode = (fun (x:nat) -> [x]);
+  encode_inj = (fun x y -> ());
+}
+
+instance integer_encodable_u8: integer_encodable FStar.UInt8.t = {
+  encode = (fun x -> [FStar.UInt8.v x]);
+  encode_inj = (fun x y -> ());
+}
+
+instance integer_encodable_u32: integer_encodable FStar.UInt32.t = {
+  encode = (fun x -> [FStar.UInt32.v x]);
+  encode_inj = (fun x y -> ());
+}
+
+instance integer_encodable_seq (t:Type) {|integer_encodable t|}: integer_encodable (Seq.seq t) = {
+  encode = (fun x -> encode (Seq.seq_to_list x));
+  encode_inj = (fun x y ->
+    assert(Seq.seq_of_list (Seq.seq_to_list x) == x);
+    assert(Seq.seq_of_list (Seq.seq_to_list y) == y);
+    encode_inj (Seq.seq_to_list x) (Seq.seq_to_list y)
+  );
+}
+
+instance integer_encodable_char: integer_encodable FStar.Char.char = {
+  encode = (fun x ->
+    encode (FStar.Char.u32_of_char x <: FStar.UInt32.t)
+  );
+  encode_inj = (fun x y ->
+    encode_inj (FStar.Char.u32_of_char x <: FStar.UInt32.t) (FStar.Char.u32_of_char y <: FStar.UInt32.t)
+  );
+}
+
+instance integer_encodable_string: integer_encodable string = {
+  encode = (fun x ->
+    encode (FStar.String.list_of_string x)
+  );
+  encode_inj = (fun x y ->
+    FStar.String.string_of_list_of_string x;
+    FStar.String.string_of_list_of_string y;
+    encode_inj (FStar.String.list_of_string x) (FStar.String.list_of_string y)
+  );
+}
